cl_initial_core builds correct types for parameters

veric/coqlib4.v
@@ -4,8 +4,6 @@ Require Import EqNat.
 Require Import msl.Coqlib2.
 Require Import Relations.
 Require Export msl.eq_dec.
-Require Import Coq.Sets.Ensembles.
-
 Lemma power_nat_divide: forall n m, two_power_nat n <= two_power_nat m -> Z.divide (two_power_nat n) (two_power_nat m).
 Proof.
   intros.
@@ -38,11 +36,6 @@ Proof.
   omega.
 Qed.
 
-Set Implicit Arguments.
-
-Definition Ensemble_join {A} (X Y Z: Ensemble A): Prop :=
-  (forall a, Z a <-> X a \/ Y a) /\ (forall a, X a -> Y a -> False).
-
 Lemma nat_of_Z_eq: forall i, nat_of_Z (Z_of_nat i) = i.
 Proof.
 intros.
@@ -64,3 +57,45 @@ Qed.
 Lemma prop_unext: forall P Q: Prop, P=Q -> (P<->Q).
 Proof. intros. subst; split; auto. Qed.
 
+Lemma list_norepet_In_In: forall {K X} a x y (l:list (K*X)),
+  list_norepet (map (@fst K X) l) -> In (a, x) l -> In (a, y) l -> x = y.
+Proof.
+  induction l; intros N Ix Iy.
+   - inv Ix.
+   - simpl in N; inv N.
+     destruct Ix.
+     + subst.
+       simpl in Iy; destruct Iy as [|Iy]; [congruence|].
+       exfalso; apply (in_map (@fst K X)) in Iy; tauto.
+     + simpl in Iy; destruct Iy as [|Iy].
+       subst. exfalso; apply (in_map (@fst K X)) in H; tauto.
+       apply IHl; auto.
+Qed.
+
+Inductive sublist {A} : list A -> list A -> Prop :=
+| sublist_nil : sublist nil nil
+| sublist_cons a l1 l2 : sublist l1 l2 -> sublist (a :: l1) (a :: l2)
+| sublist_drop a l1 l2 : sublist l1 l2 -> sublist l1 (a :: l2).
+
+Lemma sublist_In {A} (a : A) l1 l2 : sublist l1 l2 -> In a l1 -> In a l2.
+Proof.
+  intros S; induction S; intros I.
+  - inversion I.
+  - simpl in I; destruct I.
+    subst; left; auto.
+    right; auto.
+  - right; auto.
+Qed.
+
+Lemma sublist_norepet {A} (l1 l2 : list A) : sublist l1 l2 -> list_norepet l2 -> list_norepet l1.
+Proof.
+  intros S; induction S; intros N; auto.
+  - inversion N; subst; constructor; auto.
+    pose proof sublist_In a l1 l2; auto.
+  - inversion N; auto.
+Qed.
+
+Require Import Coq.Sets.Ensembles.
+
+Definition Ensemble_join {A} (X Y Z: Ensemble A): Prop :=
+  (forall a, Z a <-> X a \/ Y a) /\ (forall a, X a -> Y a -> False).
